Migrate LambdaCalculus.LocallyNameless to `grind` (#35)
* migrate to grind

* have direction of open_close match other APIs

* style

* style

* prefer simp to simp_all when possible

* a couple of free_union

Cslib/Computability/LambdaCalculus/LocallyNameless/Context.lean
@@ -4,7 +4,6 @@ Released under Apache 2.0 license as described in the file LICENSE.
 Authors: Chris Henson
 -/
 
-import Cslib.Computability.LambdaCalculus.LocallyNameless.Untyped.AesopRuleset
 import Cslib.Syntax.HasWellFormed
 import Mathlib.Data.Finset.Defs
 import Mathlib.Data.Finset.Dedup
@@ -20,19 +19,21 @@ universe u v
 
 variable {Var : Type u} {Ty : Type v} [DecidableEq Var]
 
-namespace LambdaCalculus.LocallyNameless.Stlc
+namespace LambdaCalculus.LocallyNameless
 
 /-- A typing context is a list of free variables and corresponding types. -/
 abbrev Context (Var : Type u) (Ty : Type v) := List ((_ : Var) × Ty)
 
 namespace Context
 
+open List
+
 /-- The domain of a context is the finite set of free variables it uses. -/
-@[simp]
-def dom : Context Var Ty → Finset Var := List.toFinset ∘ List.keys
+@[simp, grind =]
+def dom : Context Var Ty → Finset Var := toFinset ∘ keys
 
 /-- A well-formed context. -/
-abbrev Ok : Context Var Ty → Prop := List.NodupKeys
+abbrev Ok : Context Var Ty → Prop := NodupKeys
 
 instance : HasWellFormed (Context Var Ty) :=
   ⟨Ok⟩
@@ -40,20 +41,19 @@ instance : HasWellFormed (Context Var Ty) :=
 variable {Γ Δ : Context Var Ty}
 
 /-- Context membership is preserved on permuting a context. -/
-theorem dom_perm_mem_iff (h : Γ.Perm Δ) {x : Var} : 
-    x ∈ Γ.dom ↔ x ∈ Δ.dom := by
-  induction h <;> aesop
+theorem dom_perm_mem_iff (h : Γ.Perm Δ) {x : Var} : x ∈ Γ.dom ↔ x ∈ Δ.dom := by
+  induction h <;> simp_all only [dom, Function.comp_apply, mem_toFinset, keys_cons, mem_cons] 
+  grind
 
 omit [DecidableEq Var] in
 /-- Context well-formedness is preserved on permuting a context. -/
-@[aesop safe forward (rule_sets := [LambdaCalculus.LocallyNameless.ruleSet])]
+@[scoped grind →]
 theorem wf_perm (h : Γ.Perm Δ) : Γ✓ → Δ✓ := (List.perm_nodupKeys h).mp
 
 omit [DecidableEq Var] in
-@[aesop safe forward (rule_sets := [LambdaCalculus.LocallyNameless.ruleSet])]
-theorem wf_strengthen : (Δ ++ ⟨x, σ⟩ :: Γ)✓ → (Δ ++ Γ)✓ := by
-  intros ok
-  have sl : List.Sublist (Δ ++ Γ) (Δ ++ ⟨x, σ⟩ :: Γ) := by simp
-  exact List.NodupKeys.sublist sl ok
+/-- Context well-formedness is preserved on removing an element. -/
+@[scoped grind →]
+theorem wf_strengthen (ok : (Δ ++ ⟨x, σ⟩ :: Γ)✓) : (Δ ++ Γ)✓ := by
+  exact List.NodupKeys.sublist (by simp) ok
 
-end LambdaCalculus.LocallyNameless.Stlc.Context
+end LambdaCalculus.LocallyNameless.Context
