Cslib/Computability/LambdaCalculus/LocallyNameless/Untyped/FullBetaConfluence.lean
@@ -15,11 +15,10 @@ universe u
 
 variable {Var : Type u} 
 
-namespace LambdaCalculus.LocallyNameless.Term
+namespace LambdaCalculus.LocallyNameless.Untyped.Term
 
 /-- A parallel β-reduction step. -/
-@[aesop safe (rule_sets := [LambdaCalculus.LocallyNameless.ruleSet]) [constructors],
-  reduction_sys paraRs "ₚ"]
+@[reduction_sys paraRs "ₚ"]
 inductive Parallel : Term Var → Term Var → Prop
 /-- Free variables parallel step to themselves. -/
 | fvar (x : Var) : Parallel (fvar x) (fvar x)
@@ -34,73 +33,71 @@ inductive Parallel : Term Var → Term Var → Prop
     Parallel n n' → 
     Parallel (app (abs m) n) (m' ^ n')
 
--- TODO: I think this could be generated along with `para_rs`
-lemma para_rs_Red_eq {α} : (@paraRs α).Red = Parallel := by rfl
+open Parallel
+
+attribute [scoped grind] Parallel.fvar Parallel.app
+attribute [scoped grind cases] Parallel
 
 variable {M M' N N' : Term Var}
 
+--- TODO: I think this could be generated along with the ReductionSystem
+@[scoped grind _=_]
+private lemma para_rs_Red_eq : M ⭢ₚ N ↔ Parallel M N := by
+  have : (@paraRs Var).Red = Parallel := by rfl
+  simp_all
+
 /-- The left side of a parallel reduction is locally closed. -/
-@[aesop unsafe (rule_sets := [LambdaCalculus.LocallyNameless.ruleSet])]
+@[scoped grind]
 lemma para_lc_l (step : M ⭢ₚ N) : LC M  := by
   induction step
   case abs _ _ xs _ ih => exact LC.abs xs _ ih
   case beta => refine LC.app (LC.abs ?_ _ ?_) ?_ <;> assumption
-  all_goals constructor <;> assumption
+  all_goals grind
 
 /-- Parallel reduction is reflexive for locally closed terms. -/
-@[aesop safe (rule_sets := [LambdaCalculus.LocallyNameless.ruleSet])]
+@[scoped grind]
 lemma Parallel.lc_refl (M : Term Var) (lc : LC M) : M ⭢ₚ M := by
   induction lc
   all_goals constructor <;> assumption
 
--- TODO: better ways to handle this?
--- The problem is that sometimes when we apply a theorem we get out of our notation, so aesop can't
--- see they are the same, including constructors.
-@[aesop safe (rule_sets := [LambdaCalculus.LocallyNameless.ruleSet])]
-lemma Parallel.lc_refl' (M : Term Var) : LC M → Parallel M M := Parallel.lc_refl M
-
 variable [HasFresh Var] [DecidableEq Var]
 
 /-- The right side of a parallel reduction is locally closed. -/
-@[aesop unsafe (rule_sets := [LambdaCalculus.LocallyNameless.ruleSet])]
+@[scoped grind]
 lemma para_lc_r (step : M ⭢ₚ N) : LC N := by
   induction step
   case abs _ _ xs _ ih => exact LC.abs xs _ ih
   case beta => refine beta_lc (LC.abs ?_ _ ?_) ?_ <;> assumption
-  all_goals constructor <;> assumption
+  all_goals grind
 
 omit [HasFresh Var] [DecidableEq Var] in
 /-- A single β-reduction implies a single parallel reduction. -/
 lemma step_to_para (step : M ⭢βᶠ N) : M ⭢ₚ N := by
-  induction step <;> simp only [para_rs_Red_eq]
-  case beta _ abs_lc _ => cases abs_lc with | abs xs _ => 
-    apply Parallel.beta xs <;> intros <;> apply Parallel.lc_refl <;> aesop
-  all_goals aesop (config := {enableSimp := false})
+  induction step
+  case beta _ abs_lc _ => cases abs_lc with | abs xs _ => apply Parallel.beta xs <;> grind
+  case abs xs _ _ => apply Parallel.abs xs; grind
+  all_goals grind
 
 open FullBeta in
 /-- A single parallel reduction implies a multiple β-reduction. -/
 lemma para_to_redex (para : M ⭢ₚ N) : M ↠βᶠ N := by
   induction para
   case fvar => constructor
-  case app _ _ _ _ l_para m_para redex_l redex_m =>
-    trans
-    · exact redex_app_l_cong redex_l (para_lc_l m_para)
-    exact redex_app_r_cong redex_m (para_lc_r l_para)
+  case app L L' R R' l_para m_para redex_l redex_m =>
+    refine .trans (?_ : L.app R ↠βᶠ L'.app R) (?_ : L'.app R ↠βᶠ L'.app R') <;> grind
   case abs t t' xs _ ih =>
     apply redex_abs_cong xs
-    intros x mem
-    exact ih x mem
+    grind
   case beta m m' n n' xs para_ih para_n redex_ih redex_n =>
     have m'_abs_lc : LC m'.abs := by
       apply LC.abs xs
-      intros _ mem
-      exact para_lc_r (para_ih _ mem)
+      grind
     calc
       m.abs.app n ↠βᶠ 
       m'.abs.app n := 
         redex_app_l_cong (redex_abs_cong xs (fun _ mem ↦ redex_ih _ mem)) (para_lc_l para_n)
-      _           ↠βᶠ m'.abs.app n' := redex_app_r_cong redex_n m'_abs_lc
-      _           ⭢βᶠ m' ^ n'       := beta m'_abs_lc (para_lc_r para_n)
+      _           ↠βᶠ m'.abs.app n' := by grind
+      _           ⭢βᶠ m' ^ n'       := beta m'_abs_lc (by grind)
 
 /-- Multiple parallel reduction is equivalent to multiple β-reduction. -/
 theorem parachain_iff_redex : M ↠ₚ N ↔ M ↠βᶠ N := by
@@ -109,49 +106,27 @@ theorem parachain_iff_redex : M ↠ₚ N ↔ M ↠βᶠ N := by
   case chain_redex.tail para  redex => exact Relation.ReflTransGen.trans redex (para_to_redex para)
 
 /-- Parallel reduction respects substitution. -/
+@[scoped grind]
 lemma para_subst (x : Var) (pm : M ⭢ₚ M') (pn : N ⭢ₚ N') : M[x := N] ⭢ₚ M'[x := N'] := by
   induction pm
-  case fvar => aesop
-  case beta _ _ _ _ xs _ _ ih _ => 
-    simp only [open']
-    rw [subst_open _ _ _ _ _ (para_lc_r pn)]
-    refine Parallel.beta (xs ∪ {x}) ?_ (by assumption)
-    · intros y ymem
-      simp only [Finset.mem_union, Finset.mem_singleton, not_or] at ymem
-      push_neg at ymem
-      rw [
-        subst_def, 
-        subst_open_var _ _ _ _ _ (para_lc_r pn), 
-        subst_open_var _ _ _ _ _ (para_lc_l pn)
-      ] <;> aesop
+  case fvar => grind
+  case beta => 
+    rw [subst_open _ _ _ _ (by grind)]
+    refine Parallel.beta (free_union Var) ?_ ?_ <;> grind
   case app => constructor <;> assumption
   case abs u u' xs mem ih => 
-    apply Parallel.abs (xs ∪ {x})
-    intros y ymem
-    simp only [Finset.mem_union, Finset.mem_singleton, not_or] at ymem
-    repeat rw [subst_def]
-    push_neg at ymem
-    rw [
-      subst_open_var _ _ _ _ ?_ (para_lc_l pn), 
-      subst_open_var _ _ _ _ ?_ (para_lc_r pn)
-    ] <;> aesop
+    apply Parallel.abs (free_union Var)
+    grind
 
 /-- Parallel substitution respects closing and opening. -/
 lemma para_open_close (x y z) (para : M ⭢ₚ M') (_ : y ∉ M.fv ∪ M'.fv ∪ {x}) :
-    M⟦z ↜ x⟧⟦z ↝ fvar y⟧ ⭢ₚ M'⟦z ↜ x⟧⟦z ↝ fvar y⟧ := by
-  simp only [Finset.union_assoc, Finset.mem_union, Finset.mem_singleton, not_or] at *
-  rw [open_close_to_subst _ _ _ _ (para_lc_l para), open_close_to_subst _ _ _ _ (para_lc_r para)]
-  apply para_subst _ para
-  constructor
+    M⟦z ↜ x⟧⟦z ↝ fvar y⟧ ⭢ₚ M'⟦z ↜ x⟧⟦z ↝ fvar y⟧ := by grind
 
 /-- Parallel substitution respects fresh opening. -/
 lemma para_open_out (L : Finset Var) (mem : ∀ x, x ∉ L → (M ^ fvar x) ⭢ₚ N ^ fvar x)
     (para : M' ⭢ₚ N') : (M ^ M') ⭢ₚ (N ^ N') := by
   let ⟨x, _⟩ := fresh_exists <| free_union (map := fv) Var
-  rw [subst_intro x M' _ ?_ (para_lc_l para), subst_intro x N' _ ?_ (para_lc_r para)]
-  · refine para_subst x (mem x ?_) para
-    aesop
-  all_goals aesop
+  grind
 
 -- TODO: the Takahashi translation would be a much nicer and shorter proof, but I had difficultly
 -- writing it for locally nameless terms.
@@ -162,74 +137,60 @@ theorem para_diamond : Diamond (@Parallel Var) := by
   intros t t1 t2 tpt1
   revert t2
   induction tpt1 <;> intros t2 tpt2
-  case fvar x => exact ⟨t2, by aesop⟩
+  case fvar x => exact ⟨t2, by grind⟩
   case abs s1 s2' xs mem ih => 
     cases tpt2
     case abs t2' xs' mem' =>
-      have ⟨x, qx⟩ := fresh_exists (xs ∪ xs' ∪ t2'.fv ∪ s2'.fv)
+      have ⟨x, qx⟩ := fresh_exists (xs ∪ xs' ∪ free_union (map := fv) Var)
       simp only [Finset.union_assoc, Finset.mem_union, not_or] at qx
-      have ⟨q1, q2, q3, q4⟩ := qx
-      have ⟨t', qt'_l, qt'_r⟩ := ih x q1 (mem' _ q2)
+      have ⟨q1, q2, _⟩ := qx
+      have ⟨t', _⟩ := ih x q1 (mem' _ q2)
       exists abs (t' ^* x)
       constructor 
-      <;> [let z := s2'; let z := t2']
-      <;> apply Parallel.abs ((z ^ fvar x).fv ∪ t'.fv ∪ {x})
-      <;> intros y qy <;> simp only [open', close]
-      <;> [rw [←open_close x _ 0 q4]; rw [←open_close x _ 0 q3]] 
-      <;> refine para_open_close x y 0 ?_ qy <;> [exact qt'_l; exact qt'_r]
+      <;> [let z := s2' ^ fvar x; let z := t2' ^ fvar x]
+      <;> apply Parallel.abs (free_union (map := fv) Var) <;> grind
   case beta s1 s1' s2 s2' xs mem ps ih1 ih2 => 
     cases tpt2
     case app u2 u2' s1pu2 s2pu2' => 
       cases s1pu2
       case abs s1'' xs' mem' =>
-        have ⟨x, qx⟩ := fresh_exists (xs ∪ xs' ∪ s1''.fv ∪ s1'.fv)
+        have ⟨x, qx⟩ := fresh_exists (xs ∪ xs' ∪ free_union (map := fv) Var)
         simp only [Finset.union_assoc, Finset.mem_union, not_or] at qx
-        obtain ⟨q1, q2, q3, q4⟩ := qx
-        have ⟨t', qt'_l, qt'_r⟩ := ih2 s2pu2'
-        have ⟨t'', qt''_l, qt''_r⟩ := @ih1 x q1 _ (mem' _ q2)
+        obtain ⟨q1, q2, _⟩ := qx
+        have ⟨t', _⟩ := ih2 s2pu2'
+        have ⟨t'', _⟩ := @ih1 x q1 _ (mem' _ q2)
         exists (t'' ^* x) ^ t'
         constructor
-        · rw [subst_intro x s2' _ q4 (para_lc_l qt'_l), 
-              subst_intro x t' _ (close_var_not_fvar x t'') (para_lc_r qt'_l)]
-          simp only [open', close]
-          rw [close_open _ _ _ (para_lc_r qt''_l)]
-          exact para_subst x qt''_l qt'_l
-        · refine Parallel.beta ((s1'' ^ fvar x).fv ∪ t''.fv ∪ {x}) ?_ (by aesop)
-          intros y qy
-          rw [←open_close x s1'' 0 (by aesop)]
-          apply para_open_close <;> aesop
+        · grind
+        · apply Parallel.beta (free_union (map := fv) Var) <;> grind
     case beta u1' u2' xs' mem' s2pu2' => 
-      have ⟨x, qx⟩ := fresh_exists (xs ∪ xs' ∪ u1'.fv ∪ s1'.fv ∪ s2'.fv ∪ u2'.fv)
+      have ⟨x, qx⟩ := fresh_exists (xs ∪ xs' ∪ free_union (map := fv) Var)
       simp only [Finset.union_assoc, Finset.mem_union, not_or] at qx
-      have ⟨q1, q2, q3, q4, q5, q6⟩ := qx
-      have ⟨t', qt'_l, qt'_r⟩ := ih2 s2pu2'
-      have ⟨t'', qt''_l, qt''_r⟩ := @ih1 x q1 _ (mem' _ q2)
+      have ⟨q1, q2, _⟩ := qx
+      have ⟨t', _⟩ := ih2 s2pu2'
+      have ⟨t'', _⟩ := @ih1 x q1 _ (mem' _ q2)
       refine ⟨t'' [x := t'], ?_⟩
-      have : _ ∧ _ := ⟨para_subst x qt''_l qt'_l, para_subst x qt''_r qt'_r⟩
-      rw [subst_intro x u2' u1' _ (para_lc_l qt'_r), subst_intro x s2' s1' _ (para_lc_l qt'_l)]
-      all_goals aesop
+      grind
   case app s1 s1' s2 s2' s1ps1' _ ih1 ih2  =>
     cases tpt2
     case app u1 u2' s1 s2 =>
       have ⟨l, _, _⟩ := ih1 s1
       have ⟨r, _, _⟩ := ih2 s2
-      exact ⟨app l r, by aesop⟩
+      exact ⟨app l r, by grind⟩
     case beta t1' u1' u2' xs mem s2pu2' => 
       cases s1ps1'
       case abs s1'' xs' mem' =>
-        have ⟨x, qx⟩ := fresh_exists (xs ∪ xs' ∪ s1''.fv ∪ u1'.fv)
+        have ⟨x, qx⟩ := fresh_exists (xs ∪ xs' ∪ free_union (map := fv) Var)
         simp only [Finset.union_assoc, Finset.mem_union, not_or] at qx
-        obtain ⟨q1, q2, q3, q4⟩ := qx
+        obtain ⟨q1, q2, _⟩ := qx
         have ⟨t', qt'_l, qt'_r⟩ := ih2 s2pu2'
         have ⟨t'', qt''_l, qt''_r⟩ := @ih1 (abs u1') (Parallel.abs xs mem)
         cases qt''_l
         next w1 xs'' mem'' =>
         cases qt''_r
         case abs xs''' mem''' =>
-          exists w1 ^ t'
-          constructor
-          · aesop (config := {enableSimp := false})
-          · exact para_open_out xs''' mem''' qt'_r
+          refine ⟨w1 ^ t', ?_, para_open_out xs''' mem''' qt'_r⟩
+          apply Parallel.beta (free_union Var) <;> grind
 
 /-- Parallel reduction is confluent. -/
 theorem para_confluence : Confluence (@Parallel Var) := 
@@ -244,4 +205,4 @@ theorem confluence_beta : Confluence (@FullBeta Var) := by
   rw [←eq]
   exact @para_confluence Var _ _
 
-end LambdaCalculus.LocallyNameless.Term
+end LambdaCalculus.LocallyNameless.Untyped.Term
