Cslib/Computability/LambdaCalculus/LocallyNameless/Untyped/Properties.lean
@@ -10,79 +10,59 @@ universe u
 
 variable {Var : Type u}
 
-namespace LambdaCalculus.LocallyNameless.Term
+namespace LambdaCalculus.LocallyNameless.Untyped.Term
 
-lemma open_app_inj : app l r = (app l r)⟦i ↝ s⟧ ↔ l = l⟦i ↝ s⟧ ∧ r = r⟦i ↝ s⟧ := by
-  simp [openRec]
-
-lemma open_abs_inj : M.abs = M⟦i + 1 ↝ s⟧.abs ↔ M = M⟦i + 1 ↝ s⟧ := by
-  simp
+attribute [grind =] Finset.union_singleton 
 
 /-- An opening appearing in both sides of an equality of terms can be removed. -/
-lemma open_lc_aux (e : Term Var) : ∀ (j v i u),
-  i ≠ j →
-  e ⟦j ↝ v⟧ = (e ⟦j ↝ v⟧) ⟦i ↝ u⟧ →
-  e = e ⟦i ↝ u⟧ := by
-  induction' e <;> intros j v i u neq h 
-  case app l r ih_l ih_r => 
-    obtain ⟨hl, hr⟩ := open_app_inj.mp h
-    simp only [open_app_inj]
-    exact ⟨ih_l j v i u neq hl, ih_r j v i u neq hr⟩
-  case abs ih =>
-    simp only [openRec_abs, open_abs_inj] at *
-    exact ih (j+1) v (i+1) u (by aesop) h
-  all_goals aesop
+lemma open_lc_aux (e : Term Var) (j v i u) (neq : i ≠ j) (eq : e⟦j ↝ v⟧ = e⟦j ↝ v⟧⟦i ↝ u⟧) : 
+    e = e ⟦i ↝ u⟧ := by
+  induction e generalizing j i <;> grind
 
 /-- Opening is associative for nonclashing free variables. -/
-lemma swap_open_fvars (k n : ℕ) (x y : Var) (m : Term Var) : 
-    k ≠ n → x ≠ y → m⟦n ↝ fvar y⟧⟦k ↝ fvar x⟧ = m⟦k ↝ fvar x⟧⟦n ↝ fvar y⟧ := by
-  revert k n
-  induction' m <;> aesop
+lemma swap_open_fvars (k n : ℕ) (x y : Var) (m : Term Var) (neq : k ≠ n) : 
+    m⟦n ↝ fvar y⟧⟦k ↝ fvar x⟧ = m⟦k ↝ fvar x⟧⟦n ↝ fvar y⟧ := by
+  induction m generalizing k n <;> grind
 
 variable [DecidableEq Var]
 
 /-- Substitution of a free variable not present in a term leaves it unchanged. -/
-theorem subst_fresh (x : Var) (t sub : Term Var) : x ∉ t.fv → (t [x := sub]) = t := by
-  induction t <;> aesop
+theorem subst_fresh (x : Var) (t sub : Term Var) (nmem : x ∉ t.fv) : t [x := sub] = t := by
+  induction t <;> grind
 
 /- Opening and closing are inverses. -/
-lemma open_close (x : Var) (t : Term Var) (k : ℕ) : x ∉ t.fv → t⟦k ↝ fvar x⟧⟦k ↜ x⟧ = t := by
-  revert k
-  induction t <;> aesop
+lemma open_close (x : Var) (t : Term Var) (k : ℕ) (nmem : x ∉ t.fv) : t = t⟦k ↝ fvar x⟧⟦k ↜ x⟧ := by
+  induction t generalizing k <;> grind
 
 /-- Opening is injective. -/
 lemma open_injective (x : Var) (M M') (free_M : x ∉ M.fv) (free_M' : x ∉ M'.fv)
     (eq : M ^ fvar x = M' ^ fvar x) : M = M' := by
-  rw [←open_close x M 0 free_M, ←open_close x M' 0 free_M']
+  rw [open_close x M 0 free_M, open_close x M' 0 free_M']
   exact congrArg (closeRec 0 x) eq
 
 /-- Opening and closing are associative for nonclashing free variables. -/
-lemma swap_open_fvar_close (k n : ℕ) (x y : Var) (m : Term Var) : 
-    k ≠ n → x ≠ y → m⟦n ↝ fvar y⟧⟦k ↜ x⟧ = m⟦k ↜ x⟧⟦n ↝ fvar y⟧ := by
-  revert k n
-  induction' m <;> aesop
+lemma swap_open_fvar_close (k n : ℕ) (x y : Var) (m : Term Var) (neq₁ : k ≠ n) (neq₂ : x ≠ y) : 
+    m⟦n ↝ fvar y⟧⟦k ↜ x⟧ = m⟦k ↜ x⟧⟦n ↝ fvar y⟧ := by
+  induction m generalizing k n <;> grind
 
 /-- Closing preserves free variables. -/
-lemma close_preserve_not_fvar {k x y} (m : Term Var) : x ∉ m.fv → x ∉ (m⟦k ↜ y⟧).fv := by
-  revert k
-  induction m <;> aesop
+lemma close_preserve_not_fvar {k x y} (m : Term Var) (nmem : x ∉ m.fv) : x ∉ (m⟦k ↜ y⟧).fv := by
+  induction m generalizing k <;> grind
 
 /-- Opening to a fresh free variable preserves free variables. -/
-lemma open_fresh_preserve_not_fvar {k x y} (m : Term Var) : 
-    x ∉ m.fv → x ≠ y → x ∉ (m⟦k ↝ fvar y⟧).fv := by
-  revert k
-  induction m <;> aesop
+lemma open_fresh_preserve_not_fvar {k x y} (m : Term Var) (nmem : x ∉ m.fv) (neq : x ≠ y) :
+    x ∉ (m⟦k ↝ fvar y⟧).fv := by
+  induction m generalizing k <;> grind
 
 /-- Substitution preserves free variables. -/
-lemma subst_preserve_not_fvar {x y : Var} (m n : Term Var) : 
-    x ∉ m.fv ∪ n.fv → x ∉ (m [y := n]).fv := by
-  induction m
-  all_goals aesop
+lemma subst_preserve_not_fvar {x y : Var} (m n : Term Var) (nmem : x ∉ m.fv ∪ n.fv) : 
+    x ∉ (m [y := n]).fv := by
+  induction m <;> grind
 
 /-- Closing removes a free variable. -/
+@[scoped grind ←]
 lemma close_var_not_fvar_rec (x) (k) (t : Term Var) : x ∉ (t⟦k ↜ x⟧).fv := by
-  revert k
-  induction t <;> aesop
+  induction t generalizing k <;> grind
 
 /-- Specializes `close_var_not_fvar_rec` to first closing. -/
 lemma close_var_not_fvar (x) (t : Term Var) : x ∉ (t ^* x).fv := close_var_not_fvar_rec x 0 t
@@ -91,58 +71,50 @@ variable [HasFresh Var]
 
 omit [DecidableEq Var] in
 /-- A locally closed term is unchanged by opening. -/
-@[aesop safe (rule_sets := [LambdaCalculus.LocallyNameless.ruleSet])]
-lemma open_lc (k t) (e : Term Var) : e.LC → e = e⟦k ↝ t⟧ := by
-  intros e_lc
-  revert k
-  induction e_lc
+@[scoped grind =_]
+lemma open_lc (k t) (e : Term Var) (e_lc : e.LC) : e = e⟦k ↝ t⟧ := by
+  induction e_lc generalizing k
   case abs xs e _ ih => 
-    intros k
     simp only [openRec_abs, abs.injEq]
-    refine open_lc_aux e 0 (fvar (fresh xs)) (k+1) t ?_ ?_ <;> aesop
-  all_goals aesop
+    apply open_lc_aux e 0 (fvar (fresh xs)) (k+1) t <;> grind
+  all_goals grind
 
 /-- Substitution of a locally closed term distributes with opening. -/
-lemma subst_open (x : Var) (t : Term Var) (k : ℕ) (u e) :
-  LC t → 
-  (e ⟦ k ↝ u ⟧) [ x := t ] = (e [ x := t ]) ⟦k ↝  u [ x := t ]⟧ := by
-  revert k
-  induction' e <;> aesop
+@[scoped grind]
+lemma subst_openRec (x : Var) (t : Term Var) (k : ℕ) (u e) (lc : LC t) : 
+    (e⟦ k ↝ u ⟧)[x := t] = e[x := t]⟦k ↝  u [ x := t ]⟧ := by
+  induction e generalizing k <;> grind
 
-/-- Specialize `subst_open` to the first opening. -/
+/-- Specialize `subst_openRec` to the first opening. -/
+lemma subst_open (x : Var) (t : Term Var) (u e) (lc : LC t) : 
+    (e ^ u)[x := t] = e[x := t] ^ u [ x := t ] := by grind
+
+/-- Specialize `subst_open` to the free variables. -/
 theorem subst_open_var (x y : Var) (u e : Term Var) (neq : y ≠ x) (u_lc : LC u) : 
-    (e [y := u]) ^ fvar x = (e ^ fvar x) [y := u] := by
-  have h : (e ^ fvar x)[y:=u] = e[y:=u] ^ (fvar x)[y:=u] := subst_open y u 0 (fvar x) e u_lc
-  aesop
+    (e ^ fvar x)[y := u] = e[y := u] ^ fvar x := by grind
 
 /-- Substitution of locally closed terms is locally closed. -/
-theorem subst_lc {x : Var} {e u : Term Var} : LC e → LC u → LC (e [x := u]) := by
-  intros lc_e lc_u
-  induction lc_e 
-  case abs xs e _ ih =>
-    refine LC.abs ({x} ∪ xs) _ (?_ : ∀ y ∉ {x} ∪ xs, (e[x := u] ^ fvar y).LC)
-    intros y mem
-    rw [subst_open_var y x u e ?_ lc_u]
-    all_goals aesop
-  all_goals aesop
+@[scoped grind]
+theorem subst_lc {x : Var} {e u : Term Var} (e_lc : LC e) (u_lc : LC u) : LC (e [x := u]) := by
+  induction e_lc
+  case' abs => apply LC.abs (free_union Var)
+  all_goals grind
 
 /-- Opening to a term `t` is equivalent to opening to a free variable and substituting for `t`. -/
+@[scoped grind]
 lemma subst_intro (x : Var) (t e : Term Var) (mem : x ∉ e.fv) (t_lc : LC t) : 
-    e ^ t = (e ^ fvar x) [ x := t ] := by
-  simp only [open']
-  rw [subst_open x t 0 (fvar x) e t_lc, subst_fresh _ _ t mem]
-  aesop
+    e ^ t = (e ^ fvar x) [ x := t ] := by grind [subst_fresh]
 
 /-- Opening of locally closed terms is locally closed. -/
-theorem beta_lc {M N : Term Var} (m_lc : M.abs.LC) : LC N → LC (M ^ N) := by
+@[scoped grind ←]
+theorem beta_lc {M N : Term Var} (m_lc : M.abs.LC) (n_lc : LC N) : LC (M ^ N) := by
   cases m_lc
   case abs xs mem =>
-    intros n_lc
     have ⟨y, _⟩ := fresh_exists <| free_union (map := fv) Var
-    rw [subst_intro y N M (by aesop) (by assumption)]
-    apply subst_lc <;> aesop
+    grind
 
 /-- Opening then closing is equivalent to substitution. -/
+@[scoped grind =]
 lemma open_close_to_subst (m : Term Var) (x y : Var) (k : ℕ) (m_lc : LC m) : 
     m ⟦k ↜ x⟧⟦k ↝ fvar y⟧ = m [x := fvar y] := by
   revert k
@@ -150,31 +122,23 @@ lemma open_close_to_subst (m : Term Var) (x y : Var) (k : ℕ) (m_lc : LC m) :
   case abs xs t x_mem ih =>
     intros k
     have ⟨x', _⟩ := fresh_exists <| free_union (map := fv) Var
-    have s := subst_open_var x' x (fvar y) t (by aesop) (by constructor)
     simp only [closeRec_abs, openRec_abs, subst_abs]
-    simp only [open'] at *
-    rw [←open_close x' (t⟦k+1 ↜ x⟧⟦k+1 ↝ fvar y⟧) 0 ?f₁, ←open_close x' (t[x := fvar y]) 0 ?f₂]
-    rw [swap_open_fvars, ←swap_open_fvar_close, s, ih] <;> aesop
-    case f₁ => refine open_fresh_preserve_not_fvar _ (close_preserve_not_fvar _ ?_) ?_ <;> aesop
-    case f₂ => apply subst_preserve_not_fvar; aesop
-  all_goals aesop
+    rw [open_close x' (t⟦k+1 ↜ x⟧⟦k+1 ↝ fvar y⟧) 0 ?f₁, open_close x' (t[x := fvar y]) 0 ?f₂]
+    rw [swap_open_fvars, ←swap_open_fvar_close] <;> grind
+    case f₁ => grind [open_fresh_preserve_not_fvar, close_preserve_not_fvar]
+    case f₂ => grind [subst_preserve_not_fvar]
+  all_goals grind
 
 /-- Closing and opening are inverses. -/
-lemma close_open (x : Var) (t : Term Var) (k : ℕ) : LC t → t⟦k ↜ x⟧⟦k ↝ fvar x⟧ = t := by
-  intros lc_t
-  revert k
-  induction lc_t
+lemma close_open (x : Var) (t : Term Var) (k : ℕ) (t_lc : LC t) : t⟦k ↜ x⟧⟦k ↝ fvar x⟧ = t := by
+  induction t_lc generalizing k
   case abs xs t t_open_lc ih => 
-    intros k
     simp only [closeRec_abs, openRec_abs, abs.injEq]
     let z := t⟦k + 1 ↜ x⟧⟦k + 1 ↝ fvar x⟧
     have ⟨y, _⟩ := fresh_exists <| free_union (map := fv) Var
-    refine open_injective y _ _ (by aesop) (by aesop) ?_
-    rw [←ih y ?_ (k+1)]
-    · simp only [open']
-      rw [swap_open_fvar_close, swap_open_fvars]
-      all_goals aesop
-    aesop
-  all_goals aesop
+    refine open_injective y _ _ ?_ ?_ ?f
+    case f => rw [←ih y ?_ (k+1)] <;> grind [swap_open_fvar_close, swap_open_fvars]
+    all_goals grind
+  all_goals grind
 
-end LambdaCalculus.LocallyNameless.Term
+end LambdaCalculus.LocallyNameless.Untyped.Term
